Remove a bunch of old definitions and reorganize

Derivation.v
@@ -5,39 +5,30 @@ Require Import String.
 Require Import Parser.
 Import ListNotations.
 
-Inductive derives {g : grammar} : symbol -> list string -> parse_tree -> Prop :=
-| derivesT  : forall (tName : string),
-    derives (T tName)  [tName] (Leaf tName)
-| derivesNT : forall (ntName : string) (prod : production) (tokens : list string) (subtrees : list parse_tree),
-    In prod g /\ derivesList (rhs prod) tokens subtrees /\ lhs prod = (NT ntName) ->
-    derives (NT ntName) tokens (Node ntName subtrees)
-
-with derivesList {g : grammar} : list symbol -> list string -> list parse_tree -> Prop :=
-     | derivesNil  : derivesList nil nil nil
-     | derivesCons :
-         forall (hdRoot : symbol) (prefix : list string) (hdSubtree : parse_tree),                  
-           derives hdRoot prefix hdSubtree ->
-           
-           forall (tlRoots : list symbol) (suffix : list string) (tlSubtrees : list parse_tree),
-             derivesList tlRoots suffix tlSubtrees ->
-             
-             derivesList (hdRoot :: tlRoots) (prefix ++ suffix) (hdSubtree :: tlSubtrees).
-
-
-(* Binary version of the derives relation *)
-Inductive derives2 {g : grammar} : symbol -> list string -> Prop :=
-| derivesT2  : forall (tName : string),
-    derives2 (T tName)  [tName]
-| derivesNT2 : forall (ntName : string) (prod : production) (tokens : list string),
-    In prod g /\ derivesList2 (rhs prod) tokens /\ lhs prod = (NT ntName) ->
-    derives2 (NT ntName) tokens
-            
-with derivesList2 {g : grammar} : list symbol -> list string -> Prop :=
-     | derivesNil2  : derivesList2 nil nil
-     | derivesCons2 :
-         forall (hdRoot : symbol) (prefix : list string),
-           derives2 hdRoot prefix ->
-           
-           forall (tlRoots : list symbol) (suffix : list string),
-             derivesList2 tlRoots suffix ->
-             derivesList2 (hdRoot :: tlRoots) (prefix ++ suffix).
+Inductive derivesTree {g : grammar} : 
+  symbol -> list string -> tree -> Prop :=
+| derivesT : 
+    forall (y : string),
+      derivesTree (T y) [y] (Leaf y)
+| derivesNT : 
+    forall (x : string) 
+           (gamma : list symbol) 
+           (tokens : list string) 
+           (subtrees : forest),
+      In (NT x, gamma) g ->
+      derivesForest gamma tokens subtrees ->
+      derivesTree (NT x) tokens (Node x subtrees)
+with derivesForest {g : grammar} : 
+       list symbol -> list string -> forest -> Prop :=
+     | derivesFnil : derivesForest [] [] Fnil
+     | derivesFcons : 
+         forall (hdRoot : symbol)
+                (prefix suffix : list string)
+                (hdTree : tree)
+                (tlRoots : list symbol)
+                (tlTrees : forest),
+         derivesTree hdRoot prefix hdTree ->
+         derivesForest tlRoots suffix tlTrees ->
+         derivesForest (hdRoot :: tlRoots) 
+                       (prefix ++ suffix) 
+                       (Fcons hdTree tlTrees).
