ExampleGrammars.v
@@ -1,9 +1,9 @@
-Require Import Grammar.
-Require Import List.
+Require Import Grammar ParseTree.
+Require Import List String.
 Import ListNotations.
+Open Scope string_scope.
 
-(* Grammar 3.11 from Appel's "Modern Compiler Implementation 
-   in ML" *)
+(* Grammar 3.11 from "Modern Compiler Implementation in ML" *)
 Definition g311 : grammar :=
   [(NT "S", [T "if"; NT "E"; T "then"; NT "S"; T "else"; NT "S"]);
    (NT "S", [T "begin"; NT "S"; NT "L"]);
@@ -14,7 +14,7 @@ Definition g311 : grammar :=
    
    (NT "E", [T "num"; T "=="; T "num"])].
 
-(* Inner maps for the Grammar 3.11 parse table *)
+(* Grammar 3.11 parse table definitions *)
 
 Definition S_map :=
   SymbolMap.add
@@ -52,8 +52,39 @@ Definition g311ParseTable :=
           (NT "E") E_map
           (SymbolMap.empty (SymbolMap.t (list symbol))))).
 
+(* For testing purposes, a valid sentence in L(g311) 
+   and its derivation tree *)
+
+Definition g311Sentence1 :=
+  ["if"; "num"; "=="; "num"; "then";
+     "print"; "num"; "=="; "num";
+    "else";
+      "print"; "num"; "=="; "num"].
+
+Definition E_tree :=
+  Node "E"
+     (Fcons (Leaf "num")
+            (Fcons (Leaf "==")
+                   (Fcons (Leaf "num")
+                          Fnil))).
+
+Definition S_print_tree :=
+  Node "S"
+     (Fcons (Leaf "print")
+            (Fcons E_tree Fnil)).
+
+Definition g311ParseTree1 :=
+  Node "S"
+     (Fcons (Leaf "if")
+            (Fcons E_tree
+                   (Fcons (Leaf "then")
+                           (Fcons S_print_tree
+                                  (Fcons (Leaf "else")
+                                         (Fcons S_print_tree
+                                                Fnil)))))).
 
 (* Grammar 3.12 from the same textbook *)
+
 Definition g312 : grammar :=
   [(NT "Z", [T "d"]); 
    (NT "Z", [NT "X"; NT "Y"; NT "Z"]);
