ParseTree.v
@@ -1,68 +1,28 @@
 Require Import Grammar.
 Require Import String.
 (* Type variable seems to be cluttering up the definitions below. *)
-Inductive parse_tree {A} :=
-| Leaf : A -> parse_tree
-| Node : A -> list parse_tree -> parse_tree.
 
-Definition getRoot (tree : parse_tree) : symbol :=
-  match tree with
-  | Node ntName _ => NT ntName
-  | Leaf tName    => T tName
-  end.
+Section ParseTree.
 
-Definition isNode {A} (tree : (@parse_tree A)) : bool :=
-  match tree with
-  | Node _ _ => true
-  | Leaf _   => false
-  end.
-
-Definition isLeaf {A} (tree : (@parse_tree A)) : bool :=
-  negb (isNode tree).
-
-(* New stuff is here *)
+Variable A : Type.
 
 Inductive tree :=
-| Lf : string -> tree
-| Nd : string -> forest -> tree
+| Leaf : string -> tree
+| Node : string -> forest -> tree
 with forest :=
      | Fnil : forest
      | Fcons : tree -> forest -> forest.
 
-Fixpoint appForest xs ys :=
-  match xs with
-  | Fnil => ys
-  | Fcons t xs' => Fcons t (appForest xs' ys)
-  end.
-  
-
-Fixpoint revForest ts :=
-  match ts with
-  | Fnil => Fnil
-  | Fcons t ts' => appForest (revForest ts') (Fcons t Fnil)
+Definition isNode (tr : tree) : bool :=
+  match tr with
+  | Node _ _ => true
+  | Leaf _   => false
   end.
 
-Scheme tree_ind' := Induction for tree Sort Prop
-  with forest_ind' := Induction for forest Sort Prop.
+Definition isLeaf (tr : tree) : bool :=
+  negb (isNode tr).
 
-Require Import List.
-Import ListNotations.
+Scheme tree_mutual_ind := Induction for tree Sort Prop
+  with forest_mutual_ind := Induction for forest Sort Prop.
 
-Inductive derTree {g : grammar} : symbol -> list string -> tree -> Prop :=
-| derT : forall (y : string),
-    derTree (T y) [y] (Lf y)
-| derNT : forall (x : string) (gamma : list symbol) (tokens : list string) (subtrees : forest),
-    In (NT x, gamma) g ->
-    derForest gamma tokens subtrees ->
-    derTree (NT x) tokens (Nd x subtrees)
-with derForest {g : grammar} : list symbol -> list string -> forest -> Prop :=
-     | derFnil : derForest [] [] Fnil
-     | derFcons : forall (hdRoot : symbol)
-                         (prefix : list string)
-                         (hdSubtree : tree)
-                         (tlRoots : list symbol)
-                         (suffix : list string)
-                         (tlSubtrees : forest),
-         derTree hdRoot prefix hdSubtree ->
-         derForest tlRoots suffix tlSubtrees ->
-         derForest (hdRoot :: tlRoots) (prefix ++ suffix) (Fcons hdSubtree tlSubtrees).
+End ParseTree.
