DerivationTests.v
@@ -8,129 +8,106 @@ Require Import String.
 Import ListNotations.
 Open Scope string_scope.
 
-Definition input1 :=
-  ["if" ; "num" ; "==" ; "num" ; "then" ; "print" ; "num" ; "==" ; "num" ; "else" ; "print" ; "num" ; "==" ; "num"].
-
-Definition parseTree1 :=
-  (Node "S" [Leaf "if" ;
-             Node "E" [Leaf "num" ; Leaf "==" ; Leaf "num"] ;
-             Leaf "then" ;
-             Node "S" [Leaf "print" ;
-                       Node "E" [Leaf "num" ; Leaf "==" ; Leaf "num"]] ;
-             Leaf "else" ;
-             Node "S" [Leaf "print" ;
-                       Node "E" [Leaf "num" ; Leaf "==" ; Leaf "num"]]]).
-
 (* Manual proof of a derivation (don't do this again) *)
 Example derivesTest1 :
-  (@derives g311) (NT "S") input1 parseTree1.
+  (@derivesTree g311) (NT "S") g311Sentence1 g311ParseTree1.
 Proof.
-  apply derivesNT with (prod := (NT "S", [T "if" ; NT "E" ; T "then" ; NT "S" ; T "else" ; NT "S"])); simpl; split.
+  apply derivesNT with 
+      (x := "S")
+      (gamma := [T "if" ; NT "E" ; T "then" ; NT "S" ; T "else" ; NT "S"]).
   - left. reflexivity.
-  - split.
-    + apply derivesCons with (prefix := ["if"]).
-      * apply derivesT.
-      * apply derivesCons with (prefix := ["num" ; "==" ; "num"]).
-        { apply derivesNT with (prod := (NT "E", [T "num" ; T "==" ; T "num"])); simpl; split.
+  - apply derivesFcons with (prefix := ["if"]).
+    + apply derivesT.
+    + apply derivesFcons with (prefix := ["num" ; "==" ; "num"]).
+      * apply derivesNT with 
+            (x := "E")
+            (gamma := [T "num" ; T "==" ; T "num"]).
+        { repeat (try (left ; reflexivity) ; right). }
+        { apply derivesFcons with (prefix := ["num"]).
+          { apply derivesT. }
+          apply derivesFcons with (prefix := ["=="]).
+          { apply derivesT. }
+          apply derivesFcons with (prefix := ["num"]).
+          { apply derivesT. }
+          apply derivesFnil. }
+      * apply derivesFcons with (prefix := ["then"]).
+        { apply derivesT. }
+        apply derivesFcons with (prefix := ["print" ; "num" ; "==" ; "num"]).
+        { apply derivesNT with 
+              (x := "S")
+              (gamma := [T "print" ; NT "E"]).
           { repeat (try (left ; reflexivity) ; right). }
-          { split.
-            { apply derivesCons with (prefix := ["num"]).
-              { apply derivesT. }
-              { apply derivesCons with (prefix := ["=="]).
-                { apply derivesT. }
-                { apply derivesCons with (prefix := ["num"]).
-                  { apply derivesT. }
-                  { apply derivesNil. }}}}
-            { reflexivity. }}}
-        { apply derivesCons with (prefix := ["then"]).
+          apply derivesFcons with (prefix := ["print"]).
           { apply derivesT. }
-          { apply derivesCons with (prefix := ["print" ; "num" ; "==" ; "num"]).
-            { apply derivesNT with (prod := (NT "S", [T "print" ; NT "E"])); simpl ; split.
-              { repeat (try (left ; reflexivity) ; right). }
-              { split.
-                { apply derivesCons with (prefix := ["print"]).
-                  { apply derivesT. }
-                  { apply derivesCons with (prefix := ["num" ; "==" ; "num"]).
-                    { apply derivesNT with (prod := (NT "E", [T "num" ; T "==" ; T "num"])); simpl; split.
-                      { repeat (try (left ; reflexivity) ; right). }
-                      { split.
-                        { apply derivesCons with (prefix := ["num"]).
-                          { apply derivesT. }
-                          { apply derivesCons with (prefix := ["=="]).
-                            { apply derivesT. }
-                            { apply derivesCons with (prefix := ["num"]).
-                              { apply derivesT. }
-                              { apply derivesNil. }}}}
-                        { reflexivity. }}}
-                    { apply derivesNil. }}}
-                { reflexivity. }}}
-            { apply derivesCons with (prefix := ["else"]).
+          apply derivesFcons with (prefix := ["num" ; "==" ; "num"]).
+          { apply derivesNT with
+                (x := "E") 
+                (gamma := [T "num" ; T "==" ; T "num"]).
+            { repeat (try (left ; reflexivity) ; right). }
+            apply derivesFcons with (prefix := ["num"]).
+            { apply derivesT. }
+            apply derivesFcons with (prefix := ["=="]).
+            { apply derivesT. }
+            apply derivesFcons with (prefix := ["num"]).
+            { apply derivesT. }
+            apply derivesFnil. }
+          apply derivesFnil. }
+        apply derivesFcons with (prefix := ["else"]).
+        { apply derivesT. }
+        apply derivesFcons with (prefix := ["print" ; "num" ; "==" ; "num"]).
+        { apply derivesNT with 
+              (x := "S")
+              (gamma := [T "print" ; NT "E"]).
+          { repeat (try (left ; reflexivity) ; right). }
+          apply derivesFcons with (prefix := ["print"]).
           { apply derivesT. }
-          { apply derivesCons with (prefix := ["print" ; "num" ; "==" ; "num"]).
-            { apply derivesNT with (prod := (NT "S", [T "print" ; NT "E"])); simpl ; split.
-              { repeat (try (left ; reflexivity) ; right). }
-              { split.
-                { apply derivesCons with (prefix := ["print"]).
-                  { apply derivesT. }
-                  { apply derivesCons with (prefix := ["num" ; "==" ; "num"]).
-                    { apply derivesNT with (prod := (NT "E", [T "num" ; T "==" ; T "num"])); simpl; split.
-                      { repeat (try (left ; reflexivity) ; right). }
-                      { split.
-                        { apply derivesCons with (prefix := ["num"]).
-                          { apply derivesT. }
-                          { apply derivesCons with (prefix := ["=="]).
-                            { apply derivesT. }
-                            { apply derivesCons with (prefix := ["num"]).
-                              { apply derivesT. }
-                              { apply derivesNil. }}}}
-                        { reflexivity. }}}
-                    { apply derivesNil. }}}
-                { reflexivity. }}}
-            { apply derivesNil. }}}}}
-    + reflexivity.
+          apply derivesFcons with (prefix := ["num" ; "==" ; "num"]).
+          { apply derivesNT with 
+                (x := "E")
+                (gamma := [T "num" ; T "==" ; T "num"]).
+            { repeat (try (left ; reflexivity) ; right). }
+            apply derivesFcons with (prefix := ["num"]).
+            { apply derivesT. }
+            apply derivesFcons with (prefix := ["=="]).
+            { apply derivesT. }
+            apply derivesFcons with (prefix := ["num"]).
+            { apply derivesT. }
+            apply derivesFnil. }
+          apply derivesFnil. }
+        apply derivesFnil.
 Defined.
 
-(* A more automated proof of the same derivation. *)
+(* A (slightly) more automated proof of the same derivation. *)
 Example derivesTest2 :
-  (@derives g311) (NT "S") input1 parseTree1.
+  (@derivesTree g311) (NT "S") g311Sentence1 g311ParseTree1.
 Proof.
-  apply derivesNT with (prod := (NT "S", [T "if" ; NT "E" ; T "then" ; NT "S" ; T "else" ; NT "S"])); derCrush.
-  apply derivesCons with (prefix := ["num" ; "==" ; "num"]).
-  - apply derivesNT with (prod := (NT "E", [T "num" ; T "==" ; T "num"])); derCrush.
+  apply derivesNT with 
+      (x := "S")
+      (gamma := [T "if" ; NT "E" ; T "then" ; NT "S" ; T "else" ; NT "S"]);
+    derCrush.
+  apply derivesFcons with (prefix := ["num" ; "==" ; "num"]).
+  - apply derivesNT with 
+        (x := "E")
+        (gamma := [T "num" ; T "==" ; T "num"]); derCrush.
   - derCrush.
-    apply derivesCons with (prefix := ["print" ; "num" ; "==" ; "num"]).
-    + apply derivesNT with (prod := (NT "S", [T "print" ; NT "E"])); derCrush.
-      apply derivesCons with (prefix := ["num" ; "==" ; "num"]).
-      * apply derivesNT with (prod := (NT "E", [T "num" ; T "==" ; T "num"])); derCrush.
+    apply derivesFcons with (prefix := ["print" ; "num" ; "==" ; "num"]).
+    + apply derivesNT with 
+          (x := "S")
+          (gamma := [T "print" ; NT "E"]); derCrush.
+      apply derivesFcons with (prefix := ["num" ; "==" ; "num"]).
+      * apply derivesNT with 
+            (x := "E")
+            (gamma := [T "num" ; T "==" ; T "num"]); derCrush.
       * derCrush.
     + derCrush.
-      apply derivesCons with (prefix := ["print" ; "num" ; "==" ; "num"]).
-      * apply derivesNT with (prod := (NT "S", [T "print" ; NT "E"])); derCrush.
-        apply derivesCons with (prefix := ["num"; "=="; "num"]).
-        { apply derivesNT with (prod := (NT "E", [T "num" ; T "==" ; T "num"])); derCrush. }
-        { derCrush. }
-      * derCrush.
-Defined.
-
-(* Proof using the binary derivation relation, which doesn't include the notion
-   of a parse tree or semantic value *)
-Example derives2Test : (@derives2 g311) (NT "S") input1.
-Proof.
-  unfold input1.
-  apply derivesNT2 with (prod := (NT "S", [T "if" ; NT "E" ; T "then" ; NT "S" ; T "else" ; NT "S"])); derCrush.
-  apply derivesCons2 with (prefix := ["num" ; "==" ; "num"]).
-  - apply derivesNT2 with (prod := (NT "E", [T "num" ; T "==" ; T "num"])); derCrush.
-  - derCrush.
-    apply derivesCons2 with (prefix := ["print" ; "num" ; "==" ; "num"]).
-    + apply derivesNT2 with (prod := (NT "S", [T "print" ; NT "E"])); derCrush.
-      apply derivesCons2 with (prefix := ["num" ; "==" ; "num"]).
-      * apply derivesNT2 with (prod := (NT "E", [T "num" ; T "==" ; T "num"])); derCrush.
-      * derCrush.
-    + derCrush.
-      apply derivesCons2 with (prefix := ["print" ; "num" ; "==" ; "num"]).
-      * apply derivesNT2 with (prod := (NT "S", [T "print" ; NT "E"])); derCrush.
-        apply derivesCons2 with (prefix := ["num"; "=="; "num"]).
-        { apply derivesNT2 with (prod := (NT "E", [T "num" ; T "==" ; T "num"])); derCrush. }
-        { derCrush. }
+      apply derivesFcons with (prefix := ["print" ; "num" ; "==" ; "num"]).
+      * apply derivesNT with 
+            (x := "S")
+            (gamma := [T "print" ; NT "E"]); derCrush.
+        apply derivesFcons with (prefix := ["num"; "=="; "num"]).
+        { apply derivesNT with 
+              (x := "E")
+              (gamma := [T "num" ; T "==" ; T "num"]); derCrush. }
+        derCrush.
       * derCrush.
 Defined.
