ParserCorrectnessProofs.v
@@ -15,120 +15,25 @@ Import ListNotations.
 Open Scope list_scope.
 Open Scope string_scope.
   
-Lemma terminal_step :
-  forall (tbl   : parse_table)
-         (tName : string)
-         (token : string)
-         (gramStack' : list stack_elt)
-         (semStack  : list parse_tree)
-         (input : list string)
-         (tree : parse_tree)
-         (fuel  : nat),
-    cmpSymbol (T tName) (T token) = true ->
-    parseLoop tbl
-              (Sym (T tName) :: gramStack')
-              semStack
-              (token :: input)
-              (S fuel) = Accept tree
-    <->
-    parseLoop tbl
-              gramStack'
-              (Leaf tName :: semStack)
-              input
-              fuel = Accept tree.
+Lemma eq_sym_eq_T : 
+  forall (s s2 : string),
+    beqSym (T s) (T s2) = true <-> s = s2.
 Proof.
-  split.
-  - intros. simpl in H0.  rewrite H in H0. assumption.
-  - intros. simpl. rewrite H. assumption.
-Defined.
-
-Lemma nonterminal_step :
-  forall (tbl   : parse_table)
-         (ntName : string)
-         (gamma : list symbol)
-         (gramStack' : list stack_elt)
-         (syms : list stack_elt)
-         (gammaLength : nat)
-         (semStack  : list parse_tree)
-         (token : string)
-         (input : list string)
-         (tree : parse_tree)
-         (fuel  : nat),
-    parseTableLookup (NT ntName) (T token) tbl = Some gamma ->
-    syms = map Sym gamma ->
-    gammaLength = List.length gamma ->
-    parseLoop tbl
-              (Sym (NT ntName) :: gramStack')
-              semStack
-              (token :: input)
-              (S fuel) = Accept tree
-    <->
-    parseLoop tbl
-              (syms ++ Sep ntName gammaLength :: gramStack')
-              semStack
-              (token :: input)
-              fuel = Accept tree.
-Proof.
-  split.
-  - intros. simpl in H2.
-    rewrite H in H2. rewrite <- H0 in H2.
-    rewrite <- H1 in H2. assumption.
-  - intros. simpl.
-    rewrite H. rewrite <- H0.
-    rewrite <- H1. assumption.
-Defined.
-
-Lemma derives_singleton_list_of_NT_implies_derives_NT :
-  forall (g : grammar)
-         (ntName : string)
-         (tokens : list string),
-    (@derivesList2 g) [NT ntName] tokens ->
-    (@derives2 g) (NT ntName) tokens.
-Proof.
-  intros. inv H. inv H4.
-  rewrite app_nil_r. assumption.
-Defined.
-
-(* Come back to this *)
-Lemma ptLookup_In :
-  forall tbl g x y ys,
-    isParseTableFor tbl g ->
-    parseTableLookup x y tbl = Some ys ->
-    In (x, ys) g.
-Proof.
-  intros tbl g x y ys Htbl Hlookup.
-  destruct Htbl as [Hcomplete Hminimal].
-  unfold parseTableMinimal in Hminimal.
-  unfold parseTableLookup in Hlookup.
-Abort.
-
-Lemma eq_sym_eq_T : forall s s2,
-    cmpSymbol (T s) (T s2) = true <->
-    s = s2.
-Proof.
-  split.
-  - intros. unfold cmpSymbol in H.
-    destruct (SymbolMapFacts.eq_dec (T s) (T s2)).
-    + inv e. reflexivity.
+  split; intro H.
+  - unfold beqSym in H.
+    destruct (SymbolMapFacts.eq_dec (T s) (T s2)) as [Heq | Hneq].
+    + inv Heq; reflexivity.
     + inv H.
-  - intros. unfold cmpSymbol.
-    destruct (SymbolMapFacts.eq_dec (T s) (T s2)).
+  - unfold beqSym.
+    destruct (SymbolMapFacts.eq_dec (T s) (T s2)) as [Heq | Hneq].
     + reflexivity.
-    + exfalso. apply n. subst. reflexivity.
+    + exfalso. apply Hneq. subst. reflexivity.
 Defined.
 
-Print tree_ind'.
-
-Definition isNd tr :=
-  match tr with
-  | Lf _ => false
-  | Nd _ _ => true
-  end.
-
-Lemma nt_derives_node :
+Lemma nt_derives_Node :
   forall tbl x input fuel tree suffix,
     mkTree tbl (NT x) input fuel = (Some tree, suffix) ->
-    isNd tree = true.
+    isNode tree = true.
 Proof.
   intros. destruct fuel.
   - simpl in H. inv H.
@@ -142,18 +47,16 @@ Proof.
       * inv H.
 Defined.
 
-Definition isLf tr := negb (isNd tr).
-
 Lemma t_derives_Leaf :
   forall tbl y input fuel tree suffix,
     mkTree tbl (T y) input fuel = (Some tree, suffix) ->
-    isLf tree = true.
+    isLeaf tree = true.
 Proof.
   intros. destruct fuel.
   - inv H.
   - simpl in H. destruct input.
     + inv H.
-    + destruct (cmpSymbol (T y) (T s)).
+    + destruct (beqSym (T y) (T s)).
       * inv H. reflexivity.
       * inv H.
 Defined.
@@ -192,39 +95,39 @@ Theorem parse_correct : forall tbl g sym input tr suffix fuel,
     mkTree tbl sym input fuel = (Some tr, suffix) ->
     exists prefix,
       (prefix ++ suffix)%list = input /\
-      (@derTree g) sym prefix tr.
+      (@derivesTree g) sym prefix tr.
 Proof.
   intros.
   generalize dependent sym.
   generalize dependent input.
   generalize dependent suffix.
   generalize dependent fuel. 
-  induction tr using tree_ind' with
+  induction tr using tree_mutual_ind with
       (P := fun tr =>
               forall fuel suffix input sym,
                 mkTree tbl sym input fuel = (Some tr, suffix) ->
                 exists prefix,
                   (prefix ++ suffix)%list = input /\
-                  (@derTree g) sym prefix tr)
+                  (@derivesTree g) sym prefix tr)
       (P0 := fun subtrees =>
                forall fuel suffix input gamma,
                  mkForest tbl gamma input fuel = (Some subtrees, suffix) ->
                  exists prefix,
                    (prefix ++ suffix)%list = input /\
-                   (@derForest g) gamma prefix subtrees).
+                   (@derivesForest g) gamma prefix subtrees).
   - intros. destruct fuel.
     + inv H0.
     + destruct sym.
       * destruct input.
         { inv H0. }
         simpl in H0.
-        destruct (cmpSymbol (T s0) (T s1)) eqn:Hcmp.
+        destruct (beqSym (T s0) (T s1)) eqn:Hcmp.
         { inv H0. exists [s1]. split.
           { reflexivity. }
           apply eq_sym_eq_T in Hcmp. subst.
-          apply derT. }
+          apply derivesT. }
         inv H0.
-      * apply nt_derives_node in H0. inv H0.
+      * apply nt_derives_Node in H0. inv H0.
   - intros. destruct fuel.
     + inv H0.
     + destruct sym.
@@ -242,16 +145,16 @@ Proof.
               exists x. destruct H0. split.
               { assumption. }
               inv H1.
-              { apply derNT with (gamma := nil).
+              { apply derivesNT with (gamma := nil).
                 { apply lookup_tbl_in_grammar with (g := g)
                     in Htbl.
                   { assumption. }
                   assumption. }
-                apply derFnil. }
-              apply derNT with (gamma := (hdRoot :: tlRoots)).
+                apply derivesFnil. }
+              apply derivesNT with (gamma := (hdRoot :: tlRoots)).
               { apply lookup_tbl_in_grammar with (g := g)
                   in Htbl; assumption. }
-              apply derFcons.
+              apply derivesFcons.
               { assumption. }
               assumption. }
             inv H0. }}
@@ -262,7 +165,7 @@ Proof.
       * simpl in H0. inv H0.
         exists nil. split.
         { reflexivity. }
-        apply derFnil.
+        apply derivesFnil.
       * exfalso.
         simpl in H0.
         destruct (mkTree tbl s input fuel).
@@ -286,7 +189,7 @@ Proof.
             destruct H2. subst.
             exists (x ++ x0)%list. split.
             { rewrite app_assoc. reflexivity. }
-            apply derFcons.
+            apply derivesFcons.
             { assumption. }
             assumption. }
           inv H0. }
