ParserTactics.v
@@ -24,16 +24,11 @@ Ltac derCrush :=
   repeat match goal with
          | |- _ /\ _ => split
          | |- In _ _ => repeat (try (left ; reflexivity) ; right)
-         | |- derives (T _) _ _ => apply derivesT
-         | |- derives2 (T _) _  => apply derivesT2
-         | |- derivesList (T ?s :: _) _ _ =>
+         | |- derivesTree (T _) _ _ => apply derivesT
+         | |- derivesForest (T ?s :: _) _ _ =>
            let tName := s
-           in  apply derivesCons with (prefix := [tName])
-         | |- derivesList2 (T ?s :: _) _  =>
-           let tName := s
-           in  apply derivesCons2 with (prefix := [tName])
-         | |- derivesList [] _ _ => apply derivesNil
-         | |- derivesList2 [] _  => apply derivesNil2
+           in  apply derivesFcons with (prefix := [tName])
+         | |- derivesForest [] _ _ => apply derivesFnil
          | |- ?P = ?P => reflexivity
          | |- _ => simpl in *
          end.
