ParserTests.v
@@ -7,59 +7,7 @@ Require Import String.
 Import ListNotations.
 Open Scope string_scope.
 
-Definition input1 :=
-  ["if"; "num"; "=="; "num"; "then";
-     "print"; "num"; "=="; "num";
-    "else";
-      "print"; "num"; "=="; "num"].
-Definition parseTree1 :=
-  Node "S"
-       [Leaf "if";
-        Node "E"
-             [Leaf "num"; Leaf "=="; Leaf "num"];
-        Leaf "then";
-        Node "S"
-             [Leaf "print";
-              Node "E"
-                   [Leaf "num"; Leaf "=="; Leaf "num"]];
-        Leaf "else";
-        Node "S"
-             [Leaf "print";
-              Node "E"
-                   [Leaf "num"; Leaf "=="; Leaf "num"]]].
-
-Definition E_tree :=
-  Nd "E"
-     (Fcons (Lf "num")
-            (Fcons (Lf "==")
-                   (Fcons (Lf "num")
-                          Fnil))).
-
-Definition S_print_tree :=
-  Nd "S"
-     (Fcons (Lf "print")
-            (Fcons E_tree Fnil)).
-
-Definition parseTree2 :=
-  Nd "S"
-     (Fcons (Lf "if")
-            (Fcons E_tree
-                   (Fcons (Lf "then")
-                           (Fcons S_print_tree
-                                  (Fcons (Lf "else")
-                                         (Fcons S_print_tree
-                                                Fnil)))))).
-
-
-
 Example test1 :
-  parse g311ParseTable "S" input1 100 = Accept parseTree1.
-Proof. cbv. reflexivity. Defined.
-
-(* The new definition works, too! *)
-Example test2 :
-  mkTree g311ParseTable (NT "S") input1 100 =
-  (Some parseTree2, nil).
+  mkTree g311ParseTable (NT "S") g311Sentence1 100 =
+  (Some g311ParseTree1, nil).
 Proof. simpl. reflexivity. Defined.
-
-Compute (mkTree g311ParseTable (NT "S") input1 100).
